@prefix dc: <http://purl.org/dc/elements/1.1/> .
@prefix dct: <http://purl.org/dc/terms/> .
@prefix iso639-3: <https://iso639-3.sil.org/code/> .
@prefix owl: <http://www.w3.org/2002/07/owl#> .
@prefix skos: <http://www.w3.org/2004/02/skos/core#> .
@prefix csdls: <https://vocabs.sshopencloud.eu/vocabularies/csd-linguistic-subjects/> .
@prefix xsd: <http://www.w3.org/2001/XMLSchema#> .
@prefix tadirah: <https://vocabs.dariah.eu/tadirah/> .
@prefix rdfs: <http://www.w3.org/2000/01/rdf-schema#> .


csdls:0002 a skos:Concept ;
 skos:inScheme csdls: ;
 skos:prefLabel "annotation formats"@en ;
 skos:definition "format to represent annotations"@en ;
 skos:topConceptOf csdls: .

csdls:0003 a skos:Concept ;
 skos:inScheme csdls: ;
 skos:prefLabel "anthropological linguistics"@en ;
 skos:definition "the subfield of linguistics and anthropology which deals with the place of language in its wider social and cultural context, and its role in making and maintaining cultural practices and societal structures"@en ;
 rdfs:seeAlso <https://en.wikipedia.org/wiki/Anthropological_linguistics> ;
 skos:topConceptOf csdls: .

csdls:0004 a skos:Concept ;
 skos:inScheme csdls: ;
 skos:prefLabel "applied linguistics"@en ;
 skos:definition "an interdisciplinary field which identifies, investigates, and offers solutions to language-related real-life problems"@en ;
 rdfs:seeAlso <https://en.wikipedia.org/wiki/Applied_linguistics> ;
 skos:topConceptOf csdls: .

csdls:0005 a skos:Concept ;
 skos:inScheme csdls: ;
 skos:prefLabel "cognitive science"@en ;
 skos:definition "the interdisciplinary, scientific study of the mind and its processes"@en ;
 rdfs:seeAlso <https://en.wikipedia.org/wiki/Cognitive_science> ;
 skos:topConceptOf csdls: .

csdls:0006 a skos:Concept ;
 skos:inScheme csdls: ;
 skos:prefLabel "computational linguistics"@en ;
 skos:definition "an interdisciplinary field concerned with the computational modelling of natural language, as well as the study of appropriate computational approaches to linguistic questions"@en ;
 rdfs:seeAlso <https://en.wikipedia.org/wiki/Computational_linguistics> ;
 skos:topConceptOf csdls: .

csdls:0007 a skos:Concept ;
 skos:inScheme csdls: ;
 skos:prefLabel "dialectology"@en ;
 skos:definition "the scientific study of linguistic dialect, a sub-field of sociolinguistics"@en ;
 rdfs:seeAlso <https://en.wikipedia.org/wiki/Dialectology> ;
 skos:topConceptOf csdls: .

csdls:0008 a skos:Concept ;
 skos:inScheme csdls: ;
 skos:prefLabel "discourse analysis"@en ;
 skos:definition "analysis of (coherent) sequences of sentences, propositions, speech, or turns-at-talk"@en ;
 rdfs:seeAlso <https://en.wikipedia.org/wiki/Discourse_analysis> ;
 skos:topConceptOf csdls: .

csdls:0009 a skos:Concept ;
 skos:inScheme csdls: ;
 skos:prefLabel "forensic linguistics"@en ;
 skos:definition "the application of linguistic knowledge, methods, and insights to the forensic context of law, language, crime investigation, trial, and judicial procedure"@en ;
 rdfs:seeAlso <https://en.wikipedia.org/wiki/Forensic_linguistics> ;
 skos:broader  csdls:0004 .

csdls:0010 a skos:Concept ;
 skos:inScheme csdls: ;
 skos:prefLabel "general linguistics"@en ;
 skos:altLabel "theoretical linguistics"@en ;
 skos:definition "inquires into the nature of language and seeks to answer fundamental questions as to what language is, or what the common ground of all languages is"@en ;
 rdfs:seeAlso <https://en.wikipedia.org/wiki/Theoretical_linguistics> ;
 skos:topConceptOf csdls: .

csdls:0011 a skos:Concept ;
 skos:inScheme csdls: ;
 skos:prefLabel "historical linguistics"@en ;
 skos:altLabel "diachronic linguistics"@en ;
 skos:definition "the scientific study of language change over time."@en ;
 rdfs:seeAlso <https://en.wikipedia.org/wiki/Historical_linguistics> ;
 skos:topConceptOf csdls: .

csdls:0012 a skos:Concept ;
 skos:inScheme csdls: ;
 skos:prefLabel "history of linguistics"@en ;
 skos:definition "the study of linguistics over time"@en ;
 rdfs:seeAlso <https://en.wikipedia.org/wiki/History_of_linguistics> ;
 skos:topConceptOf csdls: .

csdls:0013 a skos:Concept ;
 skos:inScheme csdls: ;
 skos:prefLabel "language acquisition"@en ;
 skos:definition "the process by which humans acquire the capacity to perceive and comprehend language"@en ;
 rdfs:seeAlso <https://en.wikipedia.org/wiki/Language_acquisition> ;
 skos:topConceptOf csdls: .

csdls:0014 a skos:Concept ;
 skos:inScheme csdls: ;
 skos:prefLabel "language documentation"@en ;
 skos:altLabel "documentary linguistics"@en ;
 skos:definition "a subfield of linguistics which aims to describe the grammar and use of human languages."@en ;
 rdfs:seeAlso <https://en.wikipedia.org/wiki/Language_documentation> ;
 skos:topConceptOf csdls: .

csdls:0015 a skos:Concept ;
 skos:inScheme csdls: ;
 skos:prefLabel "lexicography"@en ;
 skos:definition "the study of lexicons, and the art of compiling, writing and editing dictionaries."@en ;
 rdfs:seeAlso <https://en.wikipedia.org/wiki/Lexicography> ;
 skos:topConceptOf csdls: .

csdls:0016 a skos:Concept ;
 skos:inScheme csdls: ;
 skos:prefLabel "lexicology"@en ;
 skos:definition "the branch of linguistics that analyzes the lexicon of a specific language"@en ;
 rdfs:seeAlso <https://en.wikipedia.org/wiki/Lexicology> ;
 skos:topConceptOf csdls: .

csdls:0017 a skos:Concept ;
 skos:inScheme csdls: ;
 skos:prefLabel "linguistic theories"@en ;
 skos:definition "theories about language"@en ;
 skos:topConceptOf csdls: .

csdls:0018 a skos:Concept ;
 skos:inScheme csdls: ;
 skos:prefLabel "linguistics and literature"@en ;
 skos:altLabel "philology"@en ;
 skos:definition "study of language in oral and written historical sources"@en ;
 rdfs:seeAlso <https://en.wikipedia.org/wiki/Philology> ;
 skos:topConceptOf csdls: .

csdls:0019 a skos:Concept ;
 skos:inScheme csdls: ;
 skos:prefLabel "mathematical linguistics"@en ;
 skos:altLabel "formal language theory"@en ;
 skos:definition "branch of mathematics that studies formal language <https://en.wikipedia.org/wiki/Formal_language>"@en ;
 skos:topConceptOf csdls: .

csdls:0020 a skos:Concept ;
 skos:inScheme csdls: ;
 skos:prefLabel "morphosyntax"@en ;
 skos:altLabel "morpho-syntax" ;
 skos:definition "level of linguistics that deals with properties that play a role both in syntax and morphology"@en ;
 skos:topConceptOf csdls: .

csdls:0021 a skos:Concept ;
 skos:inScheme csdls: ;
 skos:prefLabel "morphology"@en ;
 skos:definition "level of linguistics dealing with the internal structure of words"@en ;
 skos:topConceptOf csdls: .

csdls:0022 a skos:Concept ;
 skos:inScheme csdls: ;
 skos:prefLabel "neurolinguistics"@en ;
 skos:definition "the study of neural mechanisms in the human brain that control the comprehension, production, and acquisition of language"@en ;
 rdfs:seeAlso <https://en.wikipedia.org/wiki/Neurolinguistics> ;
 skos:topConceptOf csdls: .

csdls:0023 a skos:Concept ;
 skos:inScheme csdls: ;
 skos:prefLabel "onomatology"@en ;
 skos:altLabel "onomastics"@en ;
 skos:definition "the study of the etymology, history, and use of proper name"@en ;
 rdfs:seeAlso <https://en.wikipedia.org/wiki/Onomastics> ;
 skos:topConceptOf csdls: .

csdls:0024 a skos:Concept ;
 skos:inScheme csdls: ;
 skos:prefLabel "orthography"@en ;
 skos:definition "level of linguistics that deals with the writing system"@en ;
 skos:topConceptOf csdls: .

csdls:0025 a skos:Concept ;
 skos:inScheme csdls: ;
 skos:prefLabel "other"@en ;
 skos:definition "none of the other values in this domain"@en ;
 skos:topConceptOf csdls: .

csdls:0026 a skos:Concept ;
 skos:inScheme csdls: ;
 skos:prefLabel "philosophy of language"@en ;
 skos:definition "branch of philosophy that deals with the nature of language and the relations between language, language users, and the world."@en ;
 rdfs:seeAlso <https://en.wikipedia.org/wiki/Philosophy_of_language> ;
 skos:topConceptOf csdls: .

csdls:0027 a skos:Concept ;
 skos:inScheme csdls: ;
 skos:prefLabel "phonetics"@en ;
 skos:definition "level of language analysis that deals with sounds"@en ;
 skos:topConceptOf csdls: .

csdls:0028 a skos:Concept ;
 skos:inScheme csdls: ;
 skos:prefLabel "phonology"@en ;
 skos:definition "level of language analysis that describes how languages systematically organize their phones or, for sign languages, their constituent parts of signs."@en ;
 rdfs:seeAlso <https://en.wikipedia.org/wiki/Phonology> ;
 skos:topConceptOf csdls: .

csdls:0029 a skos:Concept ;
 skos:inScheme csdls: ;
 skos:prefLabel "pidgin and creole studies"@en ;
 skos:definition "branch of linguistics that studies pidgin and creole languages"@en ;
 skos:topConceptOf csdls: .

csdls:0030 a skos:Concept ;
 skos:inScheme csdls: ;
 skos:prefLabel "pragmatics"@en ;
 skos:definition "the study of how context contributes to meaning"@en ;
 rdfs:seeAlso<https://en.wikipedia.org/wiki/Pragmatics> ;
 skos:topConceptOf csdls: .

csdls:0031 a skos:Concept ;
 skos:inScheme csdls: ;
 skos:prefLabel "psycholinguistics"@en ;
 skos:definition "he study of the interrelation between linguistic factors and psychological aspects"@en ;
 rdfs:seeAlso <https://en.wikipedia.org/wiki/Psycholinguistics> ;
 skos:topConceptOf csdls: .

csdls:0032 a skos:Concept ;
 skos:inScheme csdls: ;
 skos:prefLabel "readability studies"@en ;
 skos:definition "branch of linguistics that studies readability, i.e. the ease with which a reader can understand a written text"@en ;
 rdfs:seeAlso <https://en.wikipedia.org/wiki/Readability> ;
 skos:topConceptOf csdls: .

csdls:0033 a skos:Concept ;
 skos:inScheme csdls: ;
 skos:prefLabel "semantics"@en ;
 skos:definition "level of linguistics that deals with meaning"@en ;
 skos:topConceptOf csdls: .

csdls:0034 a skos:Concept ;
 skos:inScheme csdls: ;
 skos:prefLabel "sign language"@en ;
 skos:definition "language that uses the visual-manual modality to convey meaning, instead of spoken words"@en ;
 skos:topConceptOf csdls: .

csdls:0035 a skos:Concept ;
 skos:inScheme csdls: ;
 skos:prefLabel "sociolinguistics"@en ;
 skos:definition "level of linguistic analysis that deals with the relation between language (use) and society"@en ;
 skos:topConceptOf csdls: .

csdls:0036 a skos:Concept ;
 skos:inScheme csdls: ;
 skos:prefLabel "specific language impairment studies"@en ;
 skos:altLabel "developmental language disorder studies"@en ;
 skos:definition "research that studies Specific language impairment (SLI), which is diagnosed when a child's language does not develop normally and the difficulties cannot be accounted for by generally slow development, physical abnormality of the speech apparatus, autism spectrum disorder, apraxia, acquired brain damage or hearing loss"@en ;
 rdfs:seeAlso <https://en.wikipedia.org/wiki/Specific_language_impairment> ;
 skos:topConceptOf csdls: .

csdls:0037 a skos:Concept ;
 skos:inScheme csdls: ;
 skos:prefLabel "stylistics"@en ;
 skos:definition "the study and interpretation of texts of all types and/or spoken language in regard to their linguistic and tonal style, where style is the particular variety of language used by different individuals and/or in different situations or settings"@en ;
 rdfs:seeAlso <https://en.wikipedia.org/wiki/Stylistics> ;
 skos:topConceptOf csdls: .

csdls:0038 a skos:Concept ;
 skos:inScheme csdls: ;
 skos:prefLabel "syntax"@en ;
 skos:definition "level of linguistics that deals with the combination of words and/or morphemes into larger units"@en ;
 skos:topConceptOf csdls: .

csdls:0039 a skos:Concept ;
 skos:inScheme csdls: ;
 skos:altLabel "text and corpus linguistics"@en ;
 skos:prefLabel "corpus linguistics" ;
 skos:definition "the study of a language as that language is expressed in text corpora, its bodies of 'real world' text."@en ;
 rdfs:seeAlso <https://en.wikipedia.org/wiki/Corpus_linguistics> ;
 skos:topConceptOf csdls: .

csdls:0040 a skos:Concept ;
 skos:inScheme csdls: ;
 skos:prefLabel "translating and interpreting"@en ;
 skos:definition "the activity of communicating the meaning of a textual, oral, or signed source-language  message by means of an equivalent target-language message"@en ;
 rdfs:seeAlso <https://en.wikipedia.org/wiki/Translation> ;
 skos:topConceptOf csdls: .

csdls:0041 a skos:Concept ;
 skos:inScheme csdls: ;
 skos:prefLabel "language typology"@en ;
 skos:altLabel "linguistic typology"@en ;
 skos:altLabel "typology"@en ;
 skos:definition "field of linguistics that studies and classifies languages according to their structural features to allow their comparison"@en ;
 rdfs:seeAlso <https://en.wikipedia.org/wiki/Linguistic_typology> ;
 skos:topConceptOf csdls: .

csdls:0042 a skos:Concept ;
 skos:inScheme csdls: ;
 skos:prefLabel "unknown"@en ;
 skos:definition "the value for this property is not known"@en ;
 skos:topConceptOf csdls: .

csdls:0043 a skos:Concept ;
 skos:inScheme csdls: ;
 skos:prefLabel "writing systems"@en ;
 skos:definition "A writing system is a method of visually representing verbal communication, based on a script and a set of rules regulating its use"@en ;
 rdfs:seeAlso <https://en.wikipedia.org/wiki/Writing_system> ;
 skos:topConceptOf csdls: .

csdls:0044 a skos:Concept ;
 skos:inScheme csdls: ;
 skos:prefLabel "terminology"@en ;
 skos:definition "level of linguistics that deals with terms, i.e., words or word combinations and their meanings in a specific domain"@en ;
 skos:topConceptOf csdls: .

csdls:0045 a skos:Concept ;
 skos:inScheme csdls: ;
 skos:prefLabel "discourse"@en ;
 skos:definition "level of linguistics dealing with the relations between co-occurring utterances"@en ;
 skos:topConceptOf csdls: .

csdls:0046 a skos:Concept ;
 skos:inScheme csdls: ;
 skos:prefLabel "names"@en ;
 skos:definition "expressions that identifies a single entity and that is used to refer to that entity"@en ;
 skos:topConceptOf csdls: .
 

csdls:0047 a skos:Concept ;
 skos:inScheme csdls: ;
 skos:prefLabel "multiword expressions"@en ;
 skos:definition "combinations of words that have properties that cannot be derived from the properties of the individual word nor from the rules by which they have been combined"@en ;
 skos:topConceptOf csdls: .


csdls: a skos:ConceptScheme ;
 skos:prefLabel "CLARIN Services Description Linguistic Subject taxonomy"@en ;
 dct:description "Linguistic Subject is a taxonomy of linguistic subjects used for service and tools description in the CLARIN domain"@en ;
 dc:contributor "Jan Odijk, Daan Broeder, Eline Westerhout, Rogier Kraf, Erica Renkens" ;
 dct:license <https://creativecommons.org/publicdomain/zero/1.0> ;
 dc:title "CLARIN taxonomy for Linguistic Subjects"@en ;
 dct:created "2023-08-01"^^xsd:date ;
 dct:language iso639-3:eng ;
 dct:modified "2024-01-02"^^xsd:date ;
 owl:versionInfo "1.1.0"^^xsd:string ;
 skos:hasTopConcept csdls:0002, csdls:0003,csdls:0004,csdls:0005,csdls:0006,csdls:0007,csdls:0008,csdls:0009, csdls:0010,csdls:0011,csdls:0012,csdls:0013,csdls:0014,csdls:0015,csdls:0016,csdls:0017,csdls:0018,csdls:0019, csdls:0020, csdls:0021, csdls:0022, csdls:0023, csdls:0024, csdls:0025, csdls:0026, csdls:0027, csdls:0028, csdls:0029, csdls:0030, csdls:0031,csdls:0032,csdls:0033,csdls:0034,csdls:0035,csdls:0036,csdls:0037,csdls:0038,csdls:0039, csdls:0040, csdls:0041,csdls:0042,csdls:0043 .

